finished compatibility of fseq with add & mult !!

theories/eps0_fseq.v
@@ -221,6 +221,18 @@ Section eps0_fseq.
 
   Fact eps0_fseq_fix_5 e j f l l' n : f <ε₀ ω^e → @eps0_fseq (ω^⟨e,j⟩ +₀ f) l n = ω^⟨e,j⟩ +₀ @eps0_fseq f l' n.
   Proof. solve fix. Qed.
+  
+  Fact eps0_fseq_gt_zero e (l : eps0_is_limit e) : ∀n, 0₀ <ε₀ eps0_fseq l n.
+  Proof.
+    induction l as [ e j l l' | e | e j | e l l' IH | e j l l' IH 
+                   | e j f l l' H IH ] using eps0_fseq_dep_rect; intros n.
+    + rewrite !eps0_fseq_fix_0 with (l' := l'); auto.
+    + rewrite !eps0_fseq_fix_1; auto.
+    + rewrite !eps0_fseq_fix_2; auto.
+    + rewrite !eps0_fseq_fix_3 with (l' := l); auto.
+    + rewrite !eps0_fseq_fix_4 with (l' := l); auto.
+    + rewrite !eps0_fseq_fix_5 with (l' := l); auto.
+  Qed.
 
   Fact eps0_fseq_mono e (l : eps0_is_limit e) : ∀ n m, n < m → eps0_fseq l n <ε₀ eps0_fseq l m.
   Proof.
@@ -322,75 +334,17 @@ Section eps0_fseq.
 
   Fact eps0_max u v b : u <ε₀ b → v <ε₀ b → { w | u ≤ε₀ w ∧ v ≤ε₀ w ∧ w <ε₀ b }.
   Proof. intros ? ?; destruct (eps0_le_lt_dec u v); eauto. Qed.
-
-  Fact eps0_mult_exp_is_limit a e n :
-    0₀ <ε₀ a → 0₀ <ε₀ e → eps0_is_limit (a *₀ ω^⟨e,n⟩).
-  Proof.
-    intros Ha He.
-    destruct a as [ | b i c H1 H2 ] using eps0_hnf_rect.
-    + contradict Ha; apply eps0_lt_irrefl.
-    + rewrite eps0_mult_hnf_exp; auto.
-      apply eps0_is_limit_exp_iff; left.
-      intros (-> & ->)%eps0_add_eq_zero.
-      revert He; apply eps0_lt_irrefl.
-  Qed.
-
+  
   Hint Resolve eps0_is_succ_exp_zero : core.
 
-  (* Of course, if a is 0 then a*e = 0 is not a limit ordinal
-     is the sense we use for the fundemental sequence *)
-  Fact eps0_mult_is_limit a e :
-    0₀ <ε₀ a → eps0_is_limit e → eps0_is_limit (a *₀ e).
-  Proof.
-    intros Ha.
-    induction e as [ | | e n f He Hf IHe IHf ] using eps0_hnf_pos_rect.
-    + now rewrite eps0_mult_zero_right.
-    + intros [ [] | (_ & l) ]%eps0_is_limit_exp_iff; auto.
-      rewrite eps0_mult_1add_right.
-      destruct (eps0_m1add_is_limit a l) as [ -> | ]; auto.
-      now apply eps0_lt_irrefl in Ha.
-    + intros [ (-> & H) | H ]%eps0_add_is_limit_inv.
-      * rewrite eps0_add_zero_right; apply eps0_mult_exp_is_limit; auto.
-      * rewrite eps0_mult_distr; apply eps0_add_is_limit; auto.
-  Qed.
-
-  Local Fact eps0_not_zero_lt e : e ≠ 0₀ -> 0₀ <ε₀ e.
+  Local Fact eps0_not_zero_lt e : e ≠ 0₀ → 0₀ <ε₀ e.
   Proof. intros; destruct (eps0_zero_or_pos e); now auto. Qed.
-
-  Hint Resolve eps0_not_zero_lt : core.
-
-  Fact eps0_mult_limit_limit a i b n :
-      b <ε₀ ω^a
-    → ord_is_limit n
-    → (ω^⟨a,i⟩ +₀ b) *₀ ω^⟨0₀,n⟩ = ω^⟨a,i +ₒ (1ₒ +ₒ i) *ₒ n⟩.
-  Proof.
-    intros Hb Hn.
-    rewrite <- eps0_m1add_eq, eps0_m1add_fix_2; auto.
-  Qed.
   
-  (*
+  Local Fact eps0_zero_lt_succ e : 0₀ <ε₀ e +₀ 1₀.
+  Proof. rewrite eps0_add_one_right; apply eps0_zero_lt_succ. Qed.
 
-  Fact eps0_mult_hnf_limit a i b e n f :
-      b <ε₀ ω^a
-    → f <ε₀ ω^e
-    → e ≠ 0₀
-    → eps0_is_limit (ω^⟨e,n⟩ +₀ f)
-    → (ω^⟨a,i⟩ +₀ b) *₀ (ω^⟨e,n⟩ +₀ f) = ω^a *₀ (ω^⟨e,n⟩ +₀ f).
-  Proof.
-    intros Hab Hf He1.
-    intros [ (He & H) | (-> & [He | (-> & Hn) ]) ]%eps0_is_limit_hnf; auto.
-    + rewrite eps0_mult_hnf; auto.
-        now rewrite eps0_mult_distr, eps0_mult_omega_exp.
-      * rewrite eps0_mult_hnf, eps0_mult_zero_right, !eps0_add_zero_right, eps0_mult_omega_exp; auto.
-      * (* case  (ω^a.i).n where n is limit 
-            this would give ω^a.(i.n) *)
-        rewrite eps0_add_zero_right, !eps0_mult_1add_right, eps0_m1add_fix_2, eps0_m1add_omega; auto.
-        (* if n is limit then (1+i).(1+n) = n ?? No ... *)
-        admit.
-  Admitted.
+  Hint Resolve eps0_not_zero_lt eps0_zero_lt_succ : core.
   
-  *)
-
   Hint Resolve eps0_add_incr_left 
      eps0_add_incr_right 
      eps0_lt_succ 
@@ -543,271 +497,76 @@ Section eps0_fseq.
 
   Hint Resolve eps0_zero_lt_succ eps0_is_limit_pos : core.
   
+  Fact eps0_mult_omega_limit a e :
+      eps0_is_limit e
+    → eps0_is_limit (ω^a *₀ e).
+  Proof.
+    induction 1 as [ | | e j f l l' H ] using eps0_limit_dep_rect.
+    + rewrite eps0_mult_omega_exp, eps0_add_zero_right, eps0_is_limit_exp_iff.
+      destruct (eps0_eq_dec a 0₀); auto.
+    + rewrite eps0_mult_omega_exp, eps0_is_limit_exp_iff.
+      left; now intros (? & ->)%eps0_add_eq_zero.
+    + rewrite eps0_mult_omega_hnf; auto.
+      destruct (eps0_zero_or_pos e) as [ -> | ]; auto.
+      rewrite eps0_omega_zero in H.
+      apply eps0_lt_one in H as ->.
+      now destruct l as [ [] ].
+  Qed.
   
-
-
-End eps0_fseq.
-
-Check eps0_fseq.
-Check eps0_fseq_pirr.
-Check eps0_fseq_mono.
-Check eps0_fseq_lt.
-Check eps0_fseq_limit.
-
-
-  Proof.  Qed.
-
-
-Section eps0_ltf_pos_rect.
-
-  (** Induction principle corresponding to the following building rules 
-      for ordinals below ε₀:
-
-                    e      g  e  e≠0₀  eps0_ltf g e
-        ------   ------   ----------------------------------
-          0₀      S₀ e             g +₀ ω^e
-   *)
-
-  Variables (P : ε₀ → Type)
-            (HP0 : P 0₀)
-            (HP1 : ∀ e, P e → P (S₀ e))
-            (HP2 : ∀ g e, e ≠ 0₀ → eps0_ltf g e → P g → P e → P (g +₀ ω^e)).
-
-  Theorem eps0_ltf_pos_rect e : P e.
+  (*
+  
+  (** We start with fseq (ω^a * e) *)
+  Lemma eps0_fseq_mult_omega a e (le : eps0_is_limit e) (lae : eps0_is_limit (ω^a*₀e)) :
+     ∀n, eps0_fseq lae n ≤ε₀ ω^a *₀ eps0_fseq le n.
   Proof.
-    induction e as [ | e f H IH ] using eps0_ltf_rect; auto.
-    destruct (eps0_zero_or_pos f) as [ -> | Hf ].
-    + rewrite eps0_omega_zero, eps0_add_one_right; auto.
-    + apply HP2; auto.
-      intros ->; now apply eps0_lt_irrefl in Hf.
+    revert lae.
+    induction le as
+      [ e j l l' | e | e j | e l l' IH | e j l l' IH | e j g l l' H IH ]
+      using eps0_fseq_dep_rect.
+    + rewrite eps0_mult_omega_exp.
+      intros.
+      rewrite !eps0_fseq_fix_0 with (l' := l').
+      rewrite eps0_mult_omega_exp; auto.
+    + rewrite eps0_mult_omega.
+      rewrite <- eps0_add_assoc.
+      intros.
+      rewrite !eps0_fseq_fix_1, eps0_mult_omega_exp; auto.
+    + rewrite eps0_mult_omega_exp.
+      rewrite <- eps0_add_assoc.
+      intros.
+      rewrite !eps0_fseq_fix_2, eps0_mult_distr,
+              !eps0_mult_omega_exp, eps0_add_assoc; auto.
+    + rewrite eps0_mult_omega.
+      intros.
+      assert (l'' : eps0_is_limit (a +₀ e)) by now apply eps0_add_is_limit.
+      rewrite eps0_fseq_fix_3 with (l' := l),
+              eps0_fseq_fix_3 with (l' := l''); auto.
+      rewrite eps0_mult_omega.
+      apply eps0_omega_mono_le, eps0_fseq_add.
+    + rewrite eps0_mult_omega_exp.
+      intros.
+      assert (l'' : eps0_is_limit (a +₀ e)) by now apply eps0_add_is_limit.
+      rewrite eps0_fseq_fix_4 with (l' := l),
+              eps0_fseq_fix_4 with (l' := l''); auto.
+      rewrite eps0_mult_distr, eps0_mult_omega_exp, eps0_mult_omega.
+      apply eps0_add_mono; auto.
+      apply eps0_omega_mono_le, eps0_fseq_add.
+    + destruct (eps0_zero_or_pos e) as [ -> | He ].
+      1:{ rewrite eps0_omega_zero in H.
+          apply eps0_lt_one in H.
+          destruct (proj1 l H). }
+      rewrite eps0_mult_omega_hnf; auto.
+      intros.
+      assert (l'' : eps0_is_limit (ω^a *₀ g)) by now apply eps0_mult_omega_limit.
+      rewrite eps0_fseq_fix_5 with (l' := l''),
+              eps0_fseq_fix_5 with (l' := l); auto.
+      * rewrite eps0_mult_distr, eps0_mult_omega_exp; auto.
+      * rewrite <- eps0_mult_omega; auto.
+        apply eps0_mult_mono_right; auto.
   Qed.
-
-End eps0_ltf_pos_rect.
-
-#[local] Hint Resolve eps0_is_succ_S : core.
-
-Corollary eps0_ltf_find e : eps0_is_limit e → { a : _ & { g | e = a+₀ω^g ∧ g ≠ 0₀ ∧ eps0_ltf a g } }.
-Proof.
-  destruct e as [ | | a g ] using eps0_ltf_pos_rect.
-  + now intros [ [] _ ].
-  + intros [ _ [] ]; auto.
-  + exists a, g; auto.
-Qed.
-
-Section eps0_discriminate.
-
-  Variables (P : ε₀ → Type)
-            (HP0 : P 0₀)
-            (HP1 : ∀ e, P (S₀ e))
-            (HP2 : ∀ e, eps0_is_limit e → P e).
-
-  Hint Resolve eps0_is_limit_tf : core.
-
-  Theorem eps0_discriminate e : P e.
-  Proof. destruct e using eps0_ltf_pos_rect; auto. Qed.
-
-End eps0_discriminate.
-
-(** Tailored dependent induction principle for computing the fundemental sequence *)
-
-Section eps0_fseq_dep_rect.
-
-  Variables (P : ∀e, eps0_is_limit e → Type)
-            (HP0 : ∀ g e l, eps0_ltf g (S₀ e) → @P (g +₀ ω^(S₀ e)) l)
-            (HP1 : ∀ g e l l', eps0_ltf g e → @P e l → @P (g +₀ ω^e) l').
-
-  Hint Resolve eps0_is_limit_tf : core.
-
-  Theorem eps0_fseq_dep_rect e (l : eps0_is_limit e) : P l.
-  Proof.
-    revert l.
-    destruct e as [ | e | g e H1 H2 _ _ ]
-      using eps0_ltf_pos_rect.
-    + now intros [ [] _ ].
-    + intros [ _ [] ]; eauto.
-    + induction e as [ | e | h e H3 H4 _ IH ]
-        in H1, g, H2 |- *
-        using eps0_ltf_pos_rect; intros l.
-      * now destruct H1.
-      * now apply HP0.
-      * assert (eps0_is_limit (h+₀ ω^(e))) as l' by auto.
-        apply HP1 with l'; auto.
-  Qed.
-
-End eps0_fseq_dep_rect.
-
-(** We build the fundemental sequence *)
-
-Section eps0_fseq.
-
-  Inductive eps0_fseq_gr : ε₀ → (nat → ε₀) → Prop :=
-    | eps0_fseq_gr_0 g b   : eps0_ltf g (S₀ b)
-                           → eps0_fseq_gr (g +₀ ω^(S₀ b)) (λ n, g +₀ ω^⟨b,n⟩)
-    | eps0_fseq_gr_1 g b r : eps0_is_limit b
-                           → eps0_ltf g b
-                           → eps0_fseq_gr b r
-                           → eps0_fseq_gr (g +₀ ω^b) (λ n, g +₀ ω^(r n)).
-
-  Hint Constructors eps0_fseq_gr : core.
-
-  Local Lemma eps0_fseq_gr_fun_rec e se f sf :
-    eps0_fseq_gr e se → eps0_fseq_gr f sf → e = f → ∀n, se n = sf n.
-  Proof.
-    intros H; revert H f sf.
-    induction 1 as [ g b Hs | g b r H0 Hs H1 IH1 ].
-    + induction 1 as [ g' b' Hs' | g' b' r' H0' Hs' H2 IH2 ].
-      * intros (<- & <-%eps0_succ_inj)%eps0_eq_ltf_inv; auto.
-      * intros <-%eps0_tf_fun_right; eauto.
-        destruct H0' as (_ & []); eauto.
-    + induction 1 as [ g' b' Hs' | g' b' r' H0' Hs' H2 IH2 ].
-      * intros ->%eps0_tf_fun_right; eauto.
-        destruct H0 as (_ & []); eauto.
-      * intros (<- & <-)%eps0_eq_ltf_inv; auto.
-        intro; now rewrite IH1 with (1 := H2).
-  Qed.
-
-  Lemma eps0_fseq_gr_fun e r r' : eps0_fseq_gr e r → eps0_fseq_gr e r' → ∀n, r n = r' n.
-  Proof. intros H1 H2; now apply (eps0_fseq_gr_fun_rec H1 H2). Qed.
-
-  (** We build the fundemental sequence of a limit ordinal, packed 
-      with conformity (pwc) as spec'd with eps0_fseq_gr *)
-  Definition eps0_fseq_pwc e : eps0_is_limit e → sig (eps0_fseq_gr e).
-  Proof.
-    induction 1 as [ g e l | g e l l' ? (lam & ?) ] using eps0_fseq_dep_rect.
-    + exists (λ n, g +₀ ω^⟨e,n⟩); now constructor.
-    + exists (λ n, g +₀ ω^(lam n)); constructor; auto.
-  Qed.
-
-  Definition eps0_fseq {e} (l : eps0_is_limit e) := π₁ (@eps0_fseq_pwc e l).
-
-  Fact eps0_fseq_spec e l : eps0_fseq_gr e (@eps0_fseq e l).
-  Proof. apply (proj2_sig _). Qed.
-
-  Fact eps0_fseq_pirr e (l l' : eps0_is_limit e) n : eps0_fseq l n = eps0_fseq l' n.
-  Proof. revert n; apply eps0_fseq_gr_fun with e; apply eps0_fseq_spec. Qed.
-
-  Fact eps0_fseq_fix_0 g e (l : eps0_is_limit (g +₀ ω^(S₀ e))) n :
-    eps0_ltf g (S₀ e) → eps0_fseq l n = g +₀ ω^⟨e,n⟩.
-  Proof.
-    intro.
-    revert n; apply eps0_fseq_gr_fun with (1 := eps0_fseq_spec _).
-    constructor; auto.
-  Qed.
-
-  Fact eps0_fseq_fix_1 g e (l : eps0_is_limit (g +₀ ω^e))
-                           (l' : eps0_is_limit e) n :
-    eps0_ltf g e → eps0_fseq l n = g +₀ ω^(eps0_fseq l' n).
-  Proof.
-    intros H.
-    revert n; apply eps0_fseq_gr_fun with (1 := eps0_fseq_spec _).
-    constructor; auto.
-    apply eps0_fseq_spec.
-  Qed.
-
-  Hint Resolve eps0_ltf_zero eps0_ltf_exp eps0_ltf_hnf : core.
-
-  (** The fundemental sequence is monotonic *)
-  Fact eps0_fseq_mono e (l : eps0_is_limit e) : ∀ n m, n < m → eps0_fseq l n <ε₀ eps0_fseq l m.
-  Proof.
-    induction l using eps0_fseq_dep_rect; intros n m Hnm.
-    + rewrite !eps0_fseq_fix_0; auto.
-      apply eps0_add_mono_right, eps0_exp_mono_right; auto.
-    + rewrite !eps0_fseq_fix_1 with (l' := l1); auto.
-      apply eps0_add_mono_right, eps0_omega_mono_lt; auto.
-  Qed.
-
-  Hint Resolve eps0_lt_trans eps0_add_incr eps0_add_mono_right : core.
-
-  (** Another inversion lemma, but this time
-      for the limit of the fundemental sequence
-
-      This is inversion of _ < e when e is a limit ordinal,
-      w.r.t. the fundemental sequence of e 
-
-      This has become a nice proof *)
-  Theorem eps0_lt_fseq_inv e (l : eps0_is_limit e) f : f <ε₀ e → ∃n, f <ε₀ eps0_fseq l n.
-  Proof.
-    induction l as [ g e l H | g e l l' He IHe ]
-      in f |- * using eps0_fseq_dep_rect;
-      intros [ Hf | (k & -> & Hk) ]%eps0_lt_add_inv_add.
-   + exists 0; rewrite eps0_fseq_fix_0; eauto.
-   + apply eps0_below_omega_succ_inv in Hk as (n & Hn).
-     exists n; rewrite eps0_fseq_fix_0; auto.
-   + exists 0; rewrite eps0_fseq_fix_1 with (l' := l); eauto.
-   + apply eps0_below_omega_inv in Hk as [ -> | (a & n & Ha & H) ].
-     * exists 0; rewrite eps0_fseq_fix_1 with (l' := l); auto.
-     * apply IHe in H as (i & Hi).
-       exists i; rewrite eps0_fseq_fix_1 with (l' := l); auto.
-        apply eps0_add_mono_right.
-        apply eps0_lt_trans with (1 := Ha); auto.
-        now apply eps0_exp_mono_left.
-  Qed.
-
-  (** The fundemental sequence is lesser than its limit *)
-  Theorem eps0_fseq_lt e (l : eps0_is_limit e) n : eps0_fseq l n <ε₀ e.
-  Proof.
-    induction l as [ g e l H | g e l l' He IHe ]
-      in n |- * using eps0_fseq_dep_rect.
-    + rewrite eps0_fseq_fix_0; auto. 
-      apply eps0_add_mono_right, eps0_exp_mono_left, eps0_lt_succ.
-    + rewrite eps0_fseq_fix_1 with (l' := l); auto.
-      apply eps0_add_mono_right, eps0_exp_mono_left; auto.
-  Qed.
-
-  Fact eps0_fseq_omega_succ e (l : eps0_is_limit ω^(S₀ e)) n :
-    eps0_fseq l n = ω^⟨e,n⟩.
-  Proof.
-    revert l; rewrite <- (eps0_add_zero_left ω^_); intros l.
-    rewrite eps0_fseq_fix_0; auto.
-    now rewrite eps0_add_zero_left.
-  Qed.
-
-  Fact eps0_fseq_omega_is_limit e (l : eps0_is_limit ω^e) (l' : eps0_is_limit e) n :
-    eps0_fseq l n = ω^(eps0_fseq l' n).
-  Proof.
-    revert l; rewrite <- (eps0_add_zero_left ω^_); intros l.
-    rewrite eps0_fseq_fix_1 with (l' := l'); auto.
-    now rewrite eps0_add_zero_left.
-  Qed.
-
-  Fact eps0_fseq_exp_S_one e (l : eps0_is_limit ω^⟨S₀ e,1ₚ⟩) n :
-    eps0_fseq l n = ω^⟨e,n⟩.
-  Proof. apply eps0_fseq_omega_succ. Qed.
-
-  Fact eps0_fseq_exp_S_succ e k (l : eps0_is_limit ω^⟨S₀ e,k +ₚ 1ₚ⟩) n :
-    eps0_fseq l n = ω^⟨S₀ e,k⟩ +₀ ω^⟨e,n⟩.
-  Proof.
-    revert l; rewrite <- eps0_add_exp_omega; intros l.
-    rewrite eps0_fseq_fix_0; auto.
-  Qed.
-
-  Fact eps0_fseq_exp_one_is_limit e (l : eps0_is_limit ω^⟨e,1ₚ⟩) (l' : eps0_is_limit e) n :
-    eps0_fseq l n = ω^(eps0_fseq l' n).
-  Proof. apply eps0_fseq_omega_is_limit. Qed.
-
-  Fact eps0_fseq_exp_succ_is_limit e i (l : eps0_is_limit ω^⟨e,i +ₚ 1ₚ⟩) (l' : eps0_is_limit e) n :
-    eps0_fseq l n = ω^⟨e,i⟩ +₀ ω^(eps0_fseq l' n).
-  Proof.
-    revert l; rewrite <- eps0_add_exp_omega; intros l.
-    rewrite eps0_fseq_fix_1 with (l' := l'); auto.
-  Qed.
-
-  (* Another computation for fseq :
-     fseq (ω^e.i +₀ f) n = ω^e.i + fseq f n when f < ω^e *)
-  Lemma eps0_fseq_hnf e i f (l : eps0_is_limit (ω^⟨e,i⟩ +₀ f)) (l' : eps0_is_limit f) n :
-    f <ε₀ ω^e → eps0_fseq l n = ω^⟨e,i⟩ +₀ eps0_fseq l' n.
-  Proof.
-    intros Hf; revert l.
-    induction l' as [ | g b lb ] using eps0_fseq_dep_rect; rewrite <- eps0_add_assoc; intros l.
-    + rewrite !eps0_fseq_fix_0, eps0_add_assoc; auto.
-    + rewrite !eps0_fseq_fix_1 with (l' := lb), eps0_add_assoc; auto.
-  Qed.
-
-  Hint Resolve eps0_le_refl eps0_lt_le_weak : core.
-
-  Fact eps0_max u v b : u <ε₀ b → v <ε₀ b → { w | u ≤ε₀ w ∧ v ≤ε₀ w ∧ w <ε₀ b }.
-  Proof. intros ? ?; destruct (eps0_le_lt_dec u v); eauto. Qed.
-
+  
+  *)
+  
   Fact eps0_mult_exp_is_limit a e n :
     0₀ <ε₀ a → 0₀ <ε₀ e → eps0_is_limit (a *₀ ω^⟨e,n⟩).
   Proof.
@@ -815,12 +574,10 @@ Section eps0_fseq.
     destruct a as [ | b i c H1 H2 ] using eps0_hnf_rect.
     + contradict Ha; apply eps0_lt_irrefl.
     + rewrite eps0_mult_hnf_exp; auto.
-      apply eps0_is_limit_exp.
+      apply eps0_is_limit_exp_iff; left.
       intros (-> & ->)%eps0_add_eq_zero.
       revert He; apply eps0_lt_irrefl.
   Qed.
-
-  Hint Resolve eps0_is_succ_exp_zero : core.
 
   (* Of course, if a is 0 then a*e = 0 is not a limit ordinal
      is the sense we use for the fundemental sequence *)
@@ -830,173 +587,50 @@ Section eps0_fseq.
     intros Ha.
     induction e as [ | | e n f He Hf IHe IHf ] using eps0_hnf_pos_rect.
     + now rewrite eps0_mult_zero_right.
-    + intros [_ []]; auto.
+    + intros [ [] | (_ & l) ]%eps0_is_limit_exp_iff; auto.
+      rewrite eps0_mult_1add_right.
+      destruct (eps0_m1add_is_limit a l) as [ -> | ]; auto.
+      now apply eps0_lt_irrefl in Ha.
     + intros [ (-> & H) | H ]%eps0_add_is_limit_inv.
       * rewrite eps0_add_zero_right; apply eps0_mult_exp_is_limit; auto.
       * rewrite eps0_mult_distr; apply eps0_add_is_limit; auto.
   Qed.
 
-  Fact eps0_mult_hnf_limit a i b e :
+  Fact eps0_mult_limit_limit a i b n :
       b <ε₀ ω^a
-    → eps0_is_limit e
-    → (ω^⟨a,i⟩ +₀ b) *₀ e = ω^a *₀ e.
+    → ord_is_limit n
+    → (ω^⟨a,i⟩ +₀ b) *₀ ω^⟨0₀,n⟩ = ω^⟨a,i +ₒ (1ₒ +ₒ i) *ₒ n⟩.
   Proof.
-    intros Hab.
-    induction e as [ | e n f H _ IHf ] using eps0_hnf_rect.
-    + now intros [ [] _ ].
-    + intros He.
-      unfold eps0_omega.
-      assert (e ≠ 0₀) as He'.
-      1:{ intros ->.
-          rewrite eps0_omega_zero in H.
-          apply eps0_lt_one in H as ->.
-          rewrite eps0_add_zero_right in He.
-          apply (proj2 He); auto. }
-      assert (0₀ <ε₀ e) as He''.
-      1:{ now destruct (eps0_zero_or_pos e) as [ -> | ]. }
-      apply eps0_add_is_limit_inv in He as [ (-> & _) | Hf ].
-      * rewrite !eps0_add_zero_right, eps0_mult_hnf_exp, eps0_mult_exp; auto.
-      * rewrite eps0_mult_hnf, IHf, eps0_mult_exp_hnf; auto.
+    intros Hb Hn.
+    rewrite <- eps0_m1add_eq, eps0_m1add_fix_2; auto.
   Qed.
-
-  Hint Resolve eps0_add_incr_left 
-     eps0_add_incr_right 
-     eps0_lt_succ 
-     eps0_add_is_limit eps0_is_limit_omega
-     eps0_add_mono eps0_add_mono_right : core.
-
-  (** Notice that there are examples where fseq (a+e) n < a + fseq e n
-      for instance a = ω³+ω and e = ω²
-
-      a+e = ω³+ω+ω² = ω³+ω²
-      fseq e n = fseq ω² n = ω.(n+1)
-      fseq (a+e) n = fseq (ω³+ω²) n = ω³+ω.(n+1)
-      a+(fseq e n) = ω³+ω+ω.(n+1) = ω³+ω.(n+2)
-      and hence fseq (a+e) n < fseq (a+e) n + ω = a+(fseq e n) *)
-
-  Theorem eps0_fseq_add a e (le : eps0_is_limit e) (lae : eps0_is_limit (a+₀e)) :
-     ∀n, eps0_fseq lae n ≤ε₀ a +₀ eps0_fseq le n.
+  
+  Fact eps0_mult_hnf_ord_le a i b n :
+      b <ε₀ ω^a
+    → ω^⟨a,i +ₒ (1ₒ +ₒ i) *ₒ n⟩ ≤ε₀ (ω^⟨a,i⟩ +₀ b) *₀ ω^⟨0₀,n⟩ .
   Proof.
-    revert e le lae.
-    induction a as [ | b i c Hc _ IH ] using eps0_hnf_rect.
-    + intro e; rewrite (eps0_add_zero_left e).
-      intros; rewrite eps0_add_zero_left; auto.
-      apply eps0_le_iff_lt.
-      right; apply eps0_fseq_pirr.
-    + intros e; destruct e as [ | f n g Hg _ _ ] using eps0_hnf_rect.
-      1: intros l; exfalso; now apply (proj1 l).
-      intros le.
-      destruct (eps0_lt_sdec b f) as [ b f Hbf | f | b f Hbf ].
-      * rewrite eps0_add_hnf_lt; auto.
-        intros lae j.
-        rewrite (eps0_fseq_pirr le lae); auto.
-      * rewrite eps0_add_hnf_eq; auto.
-        generalize le.
-        apply eps0_add_is_limit_iff in le
-          as [ (-> & Hf%eps0_is_limit_exp_iff) | Hg' ].
-        - rewrite !eps0_add_zero_right.
-          destruct (pos_add_is_succ i n) as (k & Hk).
-          rewrite Hk.
-          intros le lae m.
-          destruct f as [ | f | f Hf' ] using eps0_discriminate.
-          ++ easy.
-          ++ rewrite eps0_fseq_exp_S_succ.
-             destruct (pos_one_or_succ n) as [ -> | (z & ->) ].
-             ** apply pos_succ_inj in Hk as <-.
-                rewrite eps0_fseq_exp_S_one; auto.
-             ** rewrite <- pos_add_assoc in Hk.
-                apply pos_succ_inj in Hk as <-.
-                rewrite eps0_fseq_exp_S_succ, eps0_add_hnf_eq; auto.
-                apply eps0_exp_mono_left; auto.
-          ++ rewrite eps0_fseq_exp_succ_is_limit with (l' := Hf').
-             destruct (pos_one_or_succ n) as [ -> | (z & ->) ].
-             ** apply pos_succ_inj in Hk as <-.
-                rewrite eps0_fseq_exp_one_is_limit with (l' := Hf'); auto.
-             ** rewrite <- pos_add_assoc in Hk.
-                apply pos_succ_inj in Hk as <-.
-                rewrite <- eps0_add_exp,
-                           eps0_fseq_exp_succ_is_limit with (l' := Hf'),
-                          !eps0_add_assoc; auto.
-        - intros le lae m.
-          rewrite !eps0_fseq_hnf with (l' := Hg'); auto.
-          rewrite <- eps0_add_exp, !eps0_add_assoc; auto.
-      * rewrite eps0_add_assoc.
-        intros lae m.
-        generalize (eps0_add_is_limit_inv _ _ le); intros [ (-> & Hf) | Hg' ].
-        - revert le lae; rewrite !eps0_add_zero_right; intros le lae.
-          assert (eps0_is_limit (c+₀ω^⟨f,n⟩)) as l' by auto.
-          rewrite eps0_fseq_hnf with (l' := l'), eps0_add_assoc; auto.
-          apply eps0_add_below_omega; auto; apply eps0_exp_mono_left; auto.
-        - revert lae; rewrite <- (eps0_add_assoc c); intros lae.
-          assert (eps0_is_limit (c+₀ω^⟨f,n⟩+₀g)) as l' by auto.
-          rewrite eps0_fseq_hnf with (l' := l'); auto.
-          ++ rewrite eps0_add_assoc.
-             apply eps0_add_mono; auto.
-             revert l'; rewrite eps0_add_assoc; auto.
-          ++ apply eps0_add_below_omega.
-             ** apply eps0_add_below_omega; auto.
-                apply eps0_exp_mono_left; auto.
-             ** now apply eps0_lt_trans with (1 := Hg), eps0_omega_mono_lt.
+    intros Hb.
+    rewrite <- eps0_m1add_eq.
+    destruct (ord_zero_succ_limit_dec n) as [ [ -> | (k & ->) ] | Hn ].
+    + rewrite eps0_m1add_fix_1; auto.
+      apply ord_is_succ_10.
+    + rewrite eps0_m1add_fix_1; auto.
+      apply ord_is_succ_1add; auto.
+    + rewrite eps0_m1add_fix_2; auto.
   Qed.
-
-  Hint Resolve eps0_zero_lt_succ eps0_is_limit_pos : core.
-
-  (** We start with fseq (ω^a * e) *)
-  Lemma eps0_fseq_mult_omega a e (le : eps0_is_limit e) (lae : eps0_is_limit (ω^a*₀e)) :
-     ∀n, eps0_fseq lae n ≤ε₀ ω^a *₀ eps0_fseq le n.
+  
+  Hint Resolve ord_add_incr_right ord_add_incr_left : core.
+  
+  Fact ord_mult_le_special i j : j ≤ₒ i +ₒ (1ₒ +ₒ i) *ₒ j.
   Proof.
-    revert le lae.
-    induction e as [ | f n g H IHf IHg ] using eps0_hnf_rect.
-    1: intros l; exfalso; now apply (proj1 l).
-    destruct f as [ | f | f Hf ] using eps0_discriminate.
-    + rewrite eps0_omega_zero in H.
-      apply eps0_lt_one in H as ->.
-      rewrite eps0_add_zero_right; auto.
-      intros le; exfalso; apply (proj2 le); auto.
-    + rewrite eps0_mult_omega_hnf; auto.
-      intros le lae i.
-      generalize (eps0_add_is_limit_inv _ _ le); intros [ (-> & Hf) | Hg ].
-      * revert le lae. 
-        rewrite eps0_mult_zero_right, !eps0_add_zero_right, eps0_add_succ_right.
-        intros le lae.
-        destruct (pos_one_or_succ n) as [ -> | (m & ->) ].
-        - rewrite !eps0_fseq_exp_S_one, eps0_mult_omega_exp; auto.
-        - rewrite !eps0_fseq_exp_S_succ, eps0_mult_distr, 
-                  !eps0_mult_omega_exp, eps0_add_succ_right; auto.
-      * assert (eps0_is_limit (ω^(a) *₀ g)) as Hag.
-        1: apply eps0_mult_is_limit; auto.
-        rewrite eps0_fseq_hnf with (l' := Hg); auto.
-        rewrite eps0_fseq_hnf with (l' := Hag); auto.
-        - rewrite eps0_mult_distr, eps0_mult_omega_exp; auto.
-        - apply eps0_mult_below_omega with (n := 1); auto.
-          apply eps0_exp_mono_right; auto.
-    + rewrite eps0_mult_omega_hnf; auto.
-      intros le lae i.
-      generalize (eps0_add_is_limit_inv _ _ le); intros [ (-> & Hf') | Hg ].
-      * revert le lae.
-        rewrite eps0_mult_zero_right, !eps0_add_zero_right.
-        intros le lae.
-        assert (eps0_is_limit (a +₀ f)) as Haf by auto.
-        destruct (pos_one_or_succ n) as [ -> | (m & ->) ].
-        - rewrite eps0_fseq_exp_one_is_limit with (l' := Hf),
-                  eps0_fseq_exp_one_is_limit with (l' := Haf),
-                  eps0_mult_omega. 
-          apply eps0_omega_mono_le, eps0_fseq_add.
-        - rewrite eps0_fseq_exp_succ_is_limit with (l' := Hf),
-                  eps0_fseq_exp_succ_is_limit with (l' := Haf),
-                  eps0_mult_distr, eps0_mult_omega_exp, 
-                  eps0_mult_omega.
-          apply eps0_add_mono; auto.
-          apply eps0_omega_mono_le, eps0_fseq_add.
-      * assert (eps0_is_limit (ω^(a) *₀ g)) as Hag.
-        1: apply eps0_mult_is_limit; auto.
-        rewrite eps0_fseq_hnf with (l' := Hg); auto.
-        rewrite eps0_fseq_hnf with (l' := Hag); auto.
-        - rewrite eps0_mult_distr, eps0_mult_omega_exp; auto.
-        - apply eps0_mult_below_omega with (n := 1); auto.
-          apply eps0_exp_mono_right; auto.
+    apply ord_le_trans with (i +ₒ j); auto.
+    apply ord_add_mono_le; auto.
+    rewrite <- (ord_mul_one_left j) at 1.
+    apply ord_mul_mono; auto.
   Qed.
-
+ 
+  Hint Resolve ord_mult_le_special eps0_fseq_gt_zero : core.
+  
   Theorem eps0_fseq_mult a e (le : eps0_is_limit e) (lae : eps0_is_limit (a*₀e)) :
      ∀n, eps0_fseq lae n ≤ε₀ a *₀ eps0_fseq le n.
   Proof.
@@ -1005,13 +639,89 @@ Section eps0_fseq.
       rewrite eps0_mult_zero_left in lae.
       now apply (proj1 lae).
     + revert lae.
-      rewrite eps0_mult_hnf_limit; auto.
-      intros lae n.
-      apply eps0_le_trans with (1 := eps0_fseq_mult_omega _ le lae n).
-      apply eps0_mult_mono; auto.
-      apply eps0_le_trans with ω^⟨a,i⟩; auto.
-      apply eps0_exp_mono; auto.
+      induction le as 
+        [ e j l l' | e | e j | e l l' IH | e j l l' IH | e j g l l' H IH ]
+        using eps0_fseq_dep_rect.
+      * intros lae n; rewrite eps0_fseq_fix_0 with (l' := l'); revert lae.
+        destruct (eps0_zero_or_pos e) as [ -> | He ].
+        - rewrite eps0_mult_limit_limit; auto.
+          intros lae.
+          assert (l1 : ord_is_limit ((1ₒ +ₒ i) *ₒ j)).
+          1:{ apply ord_mul_is_limit_right; auto. }
+          assert (l2 : ord_is_limit (i +ₒ (1ₒ +ₒ i) *ₒ j)).
+          1:{ apply ord_is_limit_add; auto. }
+          rewrite eps0_fseq_fix_0 with (l' := l2).
+          apply eps0_le_trans with (2 := eps0_mult_hnf_ord_le _ _ _ _ Hb).
+          apply eps0_exp_mono; auto.
+          apply ord_le_trans with (1 := ord_fseq_add _ _ l1 _ _).
+          apply ord_add_mono_le; auto.
+          apply ord_fseq_mul.
+        - rewrite !eps0_mult_hnf_exp; auto.
+          intros lae.
+          rewrite eps0_fseq_fix_0 with (l' := l'); auto.
+      * rewrite eps0_mult_hnf_omega, <- eps0_add_assoc; auto.
+        intros lae n.
+        rewrite !eps0_fseq_fix_1.
+        destruct (eps0_zero_or_pos e) as [ -> | He ].
+        - rewrite eps0_add_zero_right.
+          apply eps0_le_trans with (2 := eps0_mult_hnf_ord_le _ _ _ _ Hb); auto.
+        - rewrite eps0_mult_hnf_exp; auto.
+      * rewrite eps0_mult_hnf_exp, <- eps0_add_assoc; auto.
+        intros lae n.
+        rewrite !eps0_fseq_fix_2, eps0_mult_distr,
+                 eps0_mult_hnf_exp, <- eps0_add_assoc; auto.
+        apply eps0_add_mono; auto.
+        destruct (eps0_zero_or_pos e) as [ -> | He ].
+        - rewrite eps0_add_zero_right.
+          apply eps0_le_trans with (2 := eps0_mult_hnf_ord_le _ _ _ _ Hb); auto.
+        - rewrite eps0_mult_hnf_exp; auto.
+      * destruct (eps0_zero_or_pos e) as [ -> | He ].
+        1: now destruct l as [ [] ].
+        rewrite eps0_mult_hnf_omega; auto.
+        intros lae n.
+        assert (l1: eps0_is_limit (a +₀ e))
+          by now apply eps0_add_is_limit.
+        rewrite eps0_fseq_fix_3 with (l' := l),
+                eps0_fseq_fix_3 with (l' := l1).
+        rewrite eps0_mult_hnf_omega; auto.
+        apply eps0_omega_mono_le, eps0_fseq_add.
+      * destruct (eps0_zero_or_pos e) as [ -> | He ].
+        1: now destruct l as [ [] ].
+        rewrite eps0_mult_hnf_exp; auto.
+        intros lae n.
+        assert (l1: eps0_is_limit (a +₀ e))
+          by now apply eps0_add_is_limit.
+        rewrite eps0_fseq_fix_4 with (l' := l),
+                eps0_fseq_fix_4 with (l' := l1).
+        rewrite eps0_mult_distr, eps0_mult_hnf_omega, eps0_mult_hnf_exp; auto.
+        apply eps0_add_mono, eps0_omega_mono_le, eps0_fseq_add; auto.
+      * destruct (eps0_zero_or_pos e) as [ -> | He ].
+        1:{ exfalso; rewrite eps0_omega_zero in H.
+            apply eps0_lt_one in H as ->.
+            now destruct l as [ [] ]. }
+        rewrite eps0_mult_hnf; auto.
+        intros lae n.
+        assert (l1: eps0_is_limit ((ω^⟨a,i⟩ +₀ b) *₀ g)).
+        1:{ apply eps0_add_is_limit_iff in lae as [ [C _] | ]; auto.
+            apply eps0_mult_zero_inv in C as [ C | -> ].
+            - destruct (eps0_lt_irrefl 0₀).
+              rewrite <- C at 2; auto.
+            - now destruct l as [ [] ]. }
+        apply eps0_le_trans with (1 := eps0_fseq_add _ l1 _ _).
+        rewrite eps0_fseq_fix_5 with (l' := l); auto.
+        rewrite eps0_mult_hnf; auto.
+        now apply eps0_lt_trans with (1 := eps0_fseq_lt _ _).
   Qed.
 
 End eps0_fseq.
+
+Check eps0_fseq.
+Check eps0_fseq_pirr.
+Check eps0_fseq_mono.
+Check eps0_fseq_gt_zero.
+Check eps0_fseq_lt.
+Check eps0_fseq_limit.
+Check eps0_fseq_add.
+Check eps0_fseq_mult.
+
 
